src/OSum/CtxEquiv.v
@@ -1,0 +1,356 @@
+From MyProject.src.OSum Require Export OSum.
+Require Import Autosubst.Autosubst.
+
+Module CtxEquiv.
+Print type.
+Print expr.
+
+(* inductive definition of a hole in an expr.
+ the derivative of a polynomial functor 
+ representing the syntax/constructors
+*)
+Inductive ctx_item := 
+    | ctx_appL (e : expr)
+    | ctx_appR (e : expr)
+    | ctx_lam 
+
+    | ctx_letL (e : expr)
+    | ctx_letR (e : expr)
+
+    | ctx_binOpL (op : binop) (e : expr)
+    | ctx_binOpR (op : binop) (e : expr)
+
+    | ctx_prodL (e : expr)
+    | ctx_prodR (e : expr)
+    | ctx_fst 
+    | ctx_snd
+    
+    | ctx_ifL (e e' : expr)
+    | ctx_ifM (e e' : expr)
+    | ctx_ifR (e e' : expr)
+
+    | ctx_injSig (e : expr)
+    | ctx_injVal (e : expr)
+
+    | ctx_caseOsum (e e' e'' : expr)
+    | ctx_caseSig (e e' e'' : expr)
+    | ctx_caseTrue (e e' e'' : expr)
+    | ctx_caseFalse (e e' e'' : expr)
+
+    | ctx_Tlam 
+    | ctx_Tapp
+
+    | ctx_pack
+    | ctx_unpackL (e : expr)
+    | ctx_unpackR (e : expr).
+
+(* well typed holes/context *)
+Inductive typed_ctx_item : 
+        (* which type of hole  *)
+        ctx_item -> 
+        (* type of the hole *)
+        list type -> type -> 
+        (* type of the whole *)
+        list type -> type -> 
+        Prop := 
+    
+    (* App _ e *)
+    | tp_ctx_appL G t1 t2 e :
+        typed G e t1 ->
+        typed_ctx_item (ctx_appL e)
+            G (TArrow t1 t2)
+            G (t2)
+
+    (* App f _ *)
+    | tp_ctx_appR G t1 t2 f :
+        typed G f (TArrow t1 t2) -> 
+        typed_ctx_item (ctx_appR f) 
+            G t1  
+            G t2
+
+    (* Lam _ *)
+    | tp_ctx_lam G t t' : 
+        typed_ctx_item ctx_lam 
+            (t :: G) t'
+            G (TArrow t t')
+         
+    (* let x = _ in M *) 
+    | tp_ctx_letL G t1 t2 M : 
+        typed (t1 :: G) M t2 ->
+        typed_ctx_item (ctx_letL M) 
+            G t1
+            G t2
+
+    (* let x = e in _ *)
+    | tp_ctx_letR G t1 t2 e : 
+        typed G e t1 -> 
+        typed_ctx_item (ctx_letR e)
+            (t1 :: G) t2 
+            G t2
+
+    (*  binops *)
+    (* (_ , e) *)
+    | tp_ctx_prodL G e t1 t2 : 
+        typed G e t2 -> 
+        typed_ctx_item (ctx_prodL e)
+            G t1 
+            G (TProd t1 t2)
+    
+    (* (e , _) *)
+    | tp_ctx_prodR G e t1 t2 :
+        typed G e t1 -> 
+        typed_ctx_item (ctx_prodR e)
+            G t2
+            G (TProd t1 t2)
+
+    (* fst _ *)
+    | tp_ctx_fst G t1 t2 :
+        typed_ctx_item (ctx_fst)
+            G (TProd t1 t2)
+            G t1
+    
+    (* snd _ *)
+    | tp_ctx_snd G t1 t2 : 
+        typed_ctx_item (ctx_snd)
+            G (TProd t1 t2)
+            G t2
+
+    (* if _ then e else e' *)
+    | ty_ctx_ifL G t e e' : 
+        typed G e t -> 
+        typed G e' t -> 
+        typed_ctx_item (ctx_ifL e e')
+            G TBool 
+            G t
+    
+    (* if e then _ else e' *)
+    | ty_ctx_ifM G t e e' : 
+        typed G e TBool -> 
+        typed G e' t ->
+        typed_ctx_item (ctx_ifM e e')
+            G t 
+            G t 
+
+    (* if e then e' else _ *)
+    | ty_ctx_ifR G t e e' : 
+        typed G e TBool -> 
+        typed G e' t -> 
+        typed_ctx_item (ctx_ifR e e')
+            G t 
+            G t 
+
+    (* Inj _ e *)
+    | ty_ctx_injSig G t e : 
+        typed G e t -> 
+        typed_ctx_item (ctx_injSig e)
+            G (TCase t)
+            G TOSum
+
+    (* Inj s _ *)
+    | ty_ctx_injVal G t s : 
+        typed G s (TCase t) -> 
+        typed_ctx_item (ctx_injVal s) 
+            G t 
+            G TOSum
+
+    (* case _ of e {e' | e''} *)
+    | ty_ctx_caseOsum G t t' e e' e'' :
+        typed G e (TCase t) ->
+        typed (t :: G) e' t' -> 
+        typed G e'' t' -> 
+        typed_ctx_item (ctx_caseOsum e e' e'')
+            G TOSum
+            G t'
+    
+    (* case e of _ {e' | e''} *)
+    | ty_ctx_caseSig G t t' e e' e'' : 
+        typed G e TOSum -> 
+        typed (t :: G) e' t' -> 
+        typed G e'' t' -> 
+        typed_ctx_item (ctx_caseSig e e' e'' )
+            G (TCase t)
+            G t'
+
+    (* case e of e' {_ | e''} *)
+    | ty_ctx_caseTrue G t t' e e' e'' : 
+        typed G e TOSum -> 
+        typed G e' (TCase t) -> 
+        typed G e'' t' -> 
+        typed_ctx_item (ctx_caseTrue e e' e'')
+            (t :: G) t' 
+            G t' 
+
+    (* case e of e' {e'' | _} *)
+    | ty_ctx_caseFalse G t t' e e' e'' :
+        typed G e TOSum -> 
+        typed G e' (TCase t) -> 
+        typed (t :: G) e'' t' ->
+        typed_ctx_item (ctx_caseFalse e e' e'')
+            G t' 
+            G t'
+
+    (* TLam _ *)
+    | ty_ctx_Tlam G t: 
+        typed_ctx_item ctx_Tlam 
+            (subst (ren (+1)) <$> G) t
+            G (TForall t)
+
+    (* TApp _ *)
+    | ty_ctx_Tapp G t t' : 
+        typed_ctx_item ctx_Tapp
+            G (TForall t) 
+            G t.[t'/]
+
+    
+    (* pack _  *)
+    | ty_ctx_pack G t t' : 
+        typed_ctx_item ctx_pack
+            G t.[t'/]
+            G (TExist t)
+    (* unpack x = _ in e *)
+    | ty_ctx_unpackL G t t' e : 
+        typed (t :: (subst (ren (+1)) <$> G)) e t'.[ren (+1)] ->
+        typed_ctx_item (ctx_unpackL e)
+            G (TExist t)
+            G t'
+
+    (* unpack x = e in _ *)
+    | ty_ctx_unpackR G t t' e: 
+        typed G e (TExist t) -> 
+        typed_ctx_item (ctx_unpackR e)
+            (t :: (subst (ren (+1)) <$> G)) t'.[ren (+1)]
+            G t'.
+    
+(* plug - fill the hole *)
+Definition plug_item (ctx : ctx_item) (h : expr) : expr := 
+    match ctx with 
+        | ctx_appL e => App h e 
+        | ctx_appR e => App e h 
+        | ctx_lam => Lam h 
+        | ctx_letL e => LetIn h e 
+        | ctx_letR e => LetIn e h 
+        | ctx_binOpL op e => BinOp op h e 
+        | ctx_binOpR op e => BinOp op e h 
+        | ctx_prodL e => Pair h e 
+        | ctx_prodR e => Pair e h 
+        | ctx_fst => Fst h 
+        | ctx_snd => Snd h 
+        | ctx_ifL e e' => If h e e' 
+        | ctx_ifM e e' => If e h e' 
+        | ctx_ifR e e' => If e e' h 
+        | ctx_injSig e => Inj h e 
+        | ctx_injVal e => Inj e h 
+        | ctx_caseOsum e e' e'' => CaseOf h e e' e'' 
+        | ctx_caseSig e e' e'' => CaseOf e h e' e'' 
+        | ctx_caseTrue e e' e'' => CaseOf e e' h e'' 
+        | ctx_caseFalse e e' e'' => CaseOf e e' e'' h 
+        | ctx_Tlam => TLam h 
+        | ctx_Tapp => TApp h 
+        | ctx_pack => Pack h 
+        | ctx_unpackL e => UnpackIn h e 
+        | ctx_unpackR e => UnpackIn e h 
+    end.
+
+(* build up a context from ctx_items *)
+
+Definition ctx := list ctx_item.
+
+Definition plug (K : ctx)(e : expr) : expr := foldr plug_item e K.
+
+(* pluging in a value of the right type 
+yields a well typed expression*)
+
+Lemma typed_ctx_item_typed K G t t' e :
+    typed G e t -> 
+    typed_ctx_item K G t G t' -> 
+    typed G (plug_item K e) t'.
+Proof.
+    (* all of the admits here just need weakening of contexts*)
+    intros.
+    induction H0; simpl; eauto using typed.
+    - apply Lam_typed. admit.
+    - eapply LetIn_typed. exact H0. admit.
+    - eapply CaseOf_typed. exact H0. exact H1. 2:{ exact H2. } admit.
+    - eapply TLam_typed. admit.
+    - eapply UnpackIn_typed. exact H0. admit.
+Admitted.
+
+(* a ctx is well typed if each layer is well typed *)
+Inductive typed_ctx: ctx → list type → type → list type → type → Prop :=
+  | TPCTX_nil Γ τ :
+     typed_ctx nil Γ τ Γ τ
+  | TPCTX_cons Γ1 τ1 Γ2 τ2 Γ3 τ3 k K :
+     typed_ctx_item k Γ2 τ2 Γ3 τ3 →
+     typed_ctx K Γ1 τ1 Γ2 τ2 →
+     typed_ctx (k :: K) Γ1 τ1 Γ3 τ3.
+
+Lemma typed_ctx_typed K Γ τ Γ' τ' e :
+  typed Γ e τ → typed_ctx K Γ τ Γ' τ' → typed Γ' (plug K e) τ'.
+Proof. 
+    intros.
+    induction H0.
+    - simpl. exact H.
+    - pose proof (IHtyped_ctx H).
+    eapply typed_ctx_item_typed.
+Admitted.
+
+(* definition of contextual refinement *)
+Definition reduces K e := exists v s, rtc erased_step ([plug K e],[])([of_val v],s).
+
+Definition ctx_refines (G : list type)(e e' : expr)(t : type) := 
+    (typed G e t) -> 
+    (typed G e' t) -> 
+    forall K, (
+        typed_ctx K G t [] TUnit -> 
+        reduces K e -> 
+        reduces K e'
+    ). 
+(* Definition ctx_refines (G : list type)(e e' : expr)(t : type) := 
+    (typed G e t) -> 
+    (typed G e' t) -> 
+    forall K s v, (
+        typed_ctx K G t [] TUnit -> 
+        rtc erased_step ([plug K e], []) ([of_val v], s) -> 
+        reduces K e'
+    ). *)
+
+
+Notation "Γ ⊨ e '≤ctx≤' e' : τ" :=
+  (ctx_refines Γ e e' τ) (at level 74, e, e', τ at next level).
+
+  (*  examples *)
+(* 
+Print ectx_item.
+Definition convert (K : ectx_item) : ctx_item := 
+match K with 
+| AppLCtx e => ctx_appL e
+| AppRCtx e => ctx_appR (of_val e)
+| LetInCtx e => ctx_letL e
+| TAppCtx  => ctx_Tapp
+| PackCtx => ctx_pack
+| UnpackInCtx e => ctx_unpackL e
+| PairLCtx e => ctx_p
+end. *)
+
+Example try : [] ⊨ (Bool true) ≤ctx≤ (If (Bool true) (Bool true) (Bool false)) : TBool.
+Proof.
+    unfold ctx_refines.
+    intros.
+    destruct H2.
+    destruct H2.
+    exists x. exists x0.
+    econstructor.
+    2:{ exact H2. }
+    unfold erased_step.
+    exists [].
+    econstructor.
+    3:{ econstructor. 3:{  apply IfTrue. }
+    reflexivity.
+    reflexivity.
+    }
+    -
+    admit.
+Abort.
+
+
+End CtxEquiv.
