src/OSum/binary_soundness.v
@@ -1,0 +1,46 @@
+
+From iris.proofmode Require Import proofmode.
+From iris.program_logic Require Import adequacy.
+Require Import Autosubst.Autosubst.
+
+
+From MyProject.src.OSum Require Export OSum binary_logrel binary_fundamental binary_rules.
+
+Class capabilities Σ := Cap {
+  invs :: invGpreS Σ;
+  res :: RelationResources Σ ;
+}.
+
+Definition soundness_binaryΣ : gFunctors := #[ GFunctor (authR configRA) ].
+
+(* FIXME: Really we should define a [soundnessG] as well. *)
+Global Instance inG_soundness_binaryΣ Σ : subG soundness_binaryΣ Σ → inG Σ (authR configRA).
+Proof. solve_inG. Qed.
+
+
+Lemma basic_soundness Σ `{capabilities Σ, inG Σ (authR configRA)}
+    e e' τ v s :
+  (∀ `{logrelSig Σ, configSpec Σ}, ⊢ [] ⊨ e ≤log≤ e' : τ) →
+  rtc erased_step ([e], []) ([of_val v], s) →
+  (∃ s' v', rtc erased_step ([e'], []) ([of_val v'], s')).
+Proof.
+    intros Hlog Hstep.
+    Check (adequate NotStuck e [] (fun _ _ => exists s v, rtc erased_step ([e'],[]) ([of_val v], s))).
+    cut (adequate NotStuck e [] (fun _ _ => exists s v, rtc erased_step ([e'],[]) ([of_val v], s))).
+    { destruct 1. naive_solver. }
+    eapply (wp_adequacy Σ _). simpl.
+    iIntros (Hinv ?).
+    Print binary_logrel.state_interp.
+    iExists (fun s _ => binary_logrel.state_interp s), (fun _ => True%I).
+    iSplitL.
+    iPoseProof ((Hlog _ _ )) as "Hrel".
+    iSpecialize ("Hrel" $! [][] with "[]").
+    {
+        iSplit.
+        - iExists e' ,[]. admit.
+        - iApply (@interp_env_nil _ _ _).
+    }
+    simpl.
+    replace e with e.[env_subst[]] at 2 by by asimpl.
+    
+    Check adequate.
